src/Std/Data/DTreeMap/Basic.lean
@@ -852,7 +852,6 @@ instance [Monad m] : ForM m (DTreeMap α β cmp) ((a : α) × β a) where
 
 instance : ForInNew m (DTreeMap α β cmp) ((a : α) × β a) where
   forInNew t init kcons knil := t.forInNew init (fun a b => kcons ⟨a, b⟩) knil
-  forInNew_tail := forInNew_tail (ρ := Impl α β)
 
 instance [Monad m] : ForIn m (DTreeMap α β cmp) ((a : α) × β a) where
   forIn m init f := m.forIn (fun a b acc => f ⟨a, b⟩ acc) init
