src/Std/Data/HashSet/Raw.lean
@@ -216,10 +216,7 @@ instance {m : Type v → Type w} [Monad m] : ForM m (Raw α) α where
   forM m f := m.forM f
 
 instance {m : Type v → Type w} : ForInNew m (Raw α) α where
-  forInNew m init kcons knil := ForInNew.forInNew m.inner init (fun (a, _) => kcons a) knil
-  forInNew_tail := by
-    intros _ _ _ _ _ _ _ _ _ h
-    apply forInNew_tail (ρ := HashMap.Raw α _) (h := fun (a, _) => h a)
+  forInNew m init kcons knil := m.forInNew init kcons knil
 
 instance {m : Type v → Type w} [Monad m] : ForIn m (Raw α) α where
   forIn m init f := m.forIn f init
